

	<b>MIDTERM EXAM 1</b>	
Name, Surname:	Department:	GRADE
Student No:	Course: Calculus I	
Signature:	Exam Date: 14/11/2019	

**Duration is 70 minutes. You can not use L'hopital's rule.**

1. (A) (15 pt)  $\lim_{h \rightarrow 0} \frac{(x+h)^{10} - x^{10}}{h} =$

**Solution:** This is the definition of derivative of  $y = x^{10}$ . The answer is  $10x^9$ .

(B) (15 pt)  $\lim_{x \rightarrow 0} \frac{6x}{5 \sin x + 2x} =$

**Solution:**

$$\lim_{x \rightarrow 0} \frac{6x}{5 \sin x + 2x} = 6 \frac{1}{5 \lim_{x \rightarrow 0} \frac{\sin x}{x} + 2} = \frac{6}{5 + 2}$$

(C) (15 pt)  $\lim_{x \rightarrow -\infty} \sqrt{x^2 + 3x} + x =$

**Solution:**

$$\begin{aligned} \lim_{x \rightarrow -\infty} \sqrt{x^2 + 3x} + x &= \lim_{x \rightarrow -\infty} \frac{x^2 + 3x - x^2}{\sqrt{x^2 + 3x} - x} = \lim_{x \rightarrow -\infty} \frac{3x}{|x| \sqrt{1 + \frac{3}{x}} - x} = \lim_{x \rightarrow -\infty} \frac{3x}{-x \sqrt{1 + \frac{3}{x}} - x} \\ &= \frac{3}{-\lim_{x \rightarrow -\infty} \sqrt{1 + \frac{3}{x}} - 1} = \frac{3}{-2}. \end{aligned}$$

2. (15 pt) Using **implicit derivative**, find an equation of tangent line of the curve defined by  $\frac{\pi}{2} \tan(xy) - \frac{\pi}{2} = 0$  at  $(x, y) = (\pi, \frac{1}{4})$ .

**Solution:** Take the derivative of both sides:

$$\frac{\pi}{2} (1 + \tan^2(xy))(y + xy') = 0 \implies y + xy' = 0 \implies y' = \frac{-y}{x}$$

At the given point:

$$y' = \frac{-1}{4\pi}$$

Tangent line is

$$y - \frac{1}{4} = \frac{-1}{4\pi} (x - \pi)$$

3. (15 pt) Show that the equation  $1 + \sin x = x$  has at least one solution.

**Solution:** Let  $f(x) = 1 + \sin x - x$ .  $f(0) = 1$ ,  $f(2\pi) = 1 + 0 - 2\pi$ . Since  $f(0) > 0$ ,  $f(2\pi) < 0$  and  $f$  is continuous everywhere, there is  $c \in (0, 2\pi)$  such that  $f(c) = 0$ . That is  $1 + \sin c - c = 0$ .

4. (15 pt) Find the derivative of  $f(x) = (xe^{\cos x} + 1)^3$  at  $x = \frac{\pi}{2}$ .

**Solution:**

$$f'(x) = 3(xe^{\cos x} + 1)^2(e^{\cos x} + xe^{\cos x}(-\sin x))$$

Use  $\cos \frac{\pi}{2} = 0$ ,  $\sin \frac{\pi}{2} = 1$ ,  $e^0 = 1$  to get

$$f'(\pi/2) = 3\left(\frac{\pi}{2} + 1\right)^2\left(1 - \frac{\pi}{2}\right)$$

5. (15 pt) Find the derivative of  $(f \circ g)'$  at  $x = -1$  where  $f(u) = e^{u^2+2u}$ ,  $u = g(x) = \frac{1}{x^2} - 1$ .

**Solution:**

$$f'(u) = e^{u^2+2u}(2u+2), \quad g'(x) = \frac{-2}{x^3},$$

$$g(1) = 0, \quad g'(-1) = 2, \quad f'(g(-1)) = f'(0) = 2$$

$$(f \circ g)'(-1) = f'(g(-1))g'(-1) = 4$$